dist/gcc-compatible/Hacl_Hash_Blake2b.h
@@ -68,10 +68,14 @@ typedef struct K___uint32_t__uint8_t__s
 K___uint32_t__uint8_t_;
 
 /**
-  State allocation function when there is no key
+  State allocation function when there is a key
 */
-Hacl_Hash_Blake2b_state_t
-*Hacl_Hash_Blake2b_malloc_raw(uint32_t kk, K___uint32_t__uint8_t_ key);
+Hacl_Hash_Blake2b_state_t *Hacl_Hash_Blake2b_malloc_with_key(uint8_t *k, uint32_t kk);
+
+/**
+  State allocation function when there is a key
+*/
+Hacl_Hash_Blake2b_state_t *Hacl_Hash_Blake2b_malloc(void);
 
 /**
   Re-initialization function when there is no key
@@ -87,8 +91,7 @@ Hacl_Hash_Blake2b_update(Hacl_Hash_Blake2b_state_t *state, uint8_t *chunk, uint3
 /**
   Finish function when there is no key
 */
-void
-Hacl_Hash_Blake2b_digest_raw(uint32_t kk, Hacl_Hash_Blake2b_state_t *state, uint8_t *output);
+void Hacl_Hash_Blake2b_digest(Hacl_Hash_Blake2b_state_t *state, uint8_t *output);
 
 /**
   Free state function when there is no key
