dist/gcc-compatible/Hacl_Hash_Blake2b_Simd256.h
@@ -63,10 +63,15 @@ typedef struct Hacl_Hash_Blake2b_Simd256_state_t_s
 Hacl_Hash_Blake2b_Simd256_state_t;
 
 /**
-  State allocation function when there is no key
+  State allocation function when there is a key
 */
 Hacl_Hash_Blake2b_Simd256_state_t
-*Hacl_Hash_Blake2b_Simd256_malloc_raw(uint32_t kk, K___uint32_t__uint8_t_ key);
+*Hacl_Hash_Blake2b_Simd256_malloc_with_key0(uint8_t *k, uint32_t kk);
+
+/**
+  State allocation function when there is a key
+*/
+Hacl_Hash_Blake2b_Simd256_state_t *Hacl_Hash_Blake2b_Simd256_malloc(void);
 
 /**
   Re-initialization function when there is no key
@@ -91,11 +96,7 @@ Hacl_Hash_Blake2b_Simd256_update(
   Finish function when there is no key
 */
 void
-Hacl_Hash_Blake2b_Simd256_digest_raw(
-  uint32_t kk,
-  Hacl_Hash_Blake2b_Simd256_state_t *state,
-  uint8_t *output
-);
+Hacl_Hash_Blake2b_Simd256_digest(Hacl_Hash_Blake2b_Simd256_state_t *state, uint8_t *output);
 
 /**
   Free state function when there is no key
