code/streaming/Hacl.Streaming.Functor.fst
@@ -1800,6 +1800,10 @@ let digest #index c i t t' state output l =
   assert (B.(modifies mloc h0 h7))
 #pop-options
 
+let digest_erased #index c i t t' state output l =
+  let i = index_of_state #index c i t t' state in
+  digest #index c i t t' state output l
+
 let free #index c i t t' state =
   let _ = allow_inversion key_management in
   let open LowStar.BufferOps in
